proof

solution.v
@@ -1,7 +1,8 @@
 Require Import
   Ssreflect.ssreflect Ssreflect.ssrfun Ssreflect.ssrbool Ssreflect.eqtype
   Ssreflect.ssrnat Ssreflect.seq Ssreflect.fintype
-  MathComp.bigop MathComp.finset MathComp.fingroup MathComp.perm.
+  MathComp.path MathComp.fingraph MathComp.bigop MathComp.finset
+  MathComp.fingroup MathComp.perm.
 
 Set Implicit Arguments.
 Unset Strict Implicit.
@@ -22,23 +23,37 @@ Definition empty_space : elemt :=
 
 Definition puzzle_next (b : board) : {set board} :=
   let (ex, ey) := b^-1%g empty_space in
-  [set perm_mul b (tperm (ex, ey) npos) |
+  [set (b * tperm npos (ex, ey))%g |
     npos : elemt &
-    (npos \in [:: (inord ex.-1, ey); (inord ex.-1, ey);
+    (npos \in [:: (inord ex.-1, ey); (inord ex.+1, ey);
                   (ex, inord ey.-1); (ex, inord ey.+1)]) &&
     (npos != (ex, ey))].
 
-(*
-Definition puzzle_next' (b : board) : {set board} :=
-  let (ex, ey) := b^-1%g empty_space in
-  [set perm_mul b (tperm (ex, ey) (ex', ey')) |
-    ex' in 'I_x, ey' in 'I_y & odd (ex' + ex) (+) odd (ey' + ey)].
-*)
+Definition puzzle_reachable : rel board :=
+  connect (fun b1 b2 => b2 \in puzzle_next b1).
 
 Definition invariant (b : board) : bool :=
   let (ex, ey) := b^-1%g empty_space in
-  odd_perm b (+) odd x' (+) odd y' (+) odd ex (+) odd ey.
+  ~~ (odd_perm b (+) odd x' (+) odd y' (+) odd ex (+) odd ey).
 
+Lemma invariant1 : invariant 1.
+Proof.
+  rewrite /invariant invg1 perm1 /empty_space /= odd_perm1 /=.
+  by do 2 case: (odd _) => /=.
+Qed.
 
+Lemma invariant2 b1 b2 :
+  b2 \in puzzle_next b1 -> invariant b1 -> invariant b2.
+Proof.
+  rewrite /puzzle_next /invariant.
+  move: {1 3 4}((b1^-1)%g _) {1 3}((b2^-1)%g _)
+    (erefl ((b1^-1)%g empty_space)) (erefl ((b2^-1)%g empty_space)) =>
+    /= [] b1x b1y [] b2x b2y Hb1 Hb2.
+  case/imsetP => npos; rewrite !inE.
+  case/andP; do !case/orP; move/eqP => ?;
+    subst npos => H ?; subst b2 => /=; apply contra;
+    rewrite odd_permM odd_tperm H /=;
+    rewrite eqE /= eqxx ?andbT /= in H.
+Abort.
 
 End puzzle.
